restructure

code/k256/Hacl.K256.ECDSA.fst
@@ -11,198 +11,20 @@ module ST = FStar.HyperStack.ST
 module LSeq = Lib.Sequence
 module BSeq = Lib.ByteSequence
 
-module BD = Hacl.Bignum.Definitions
-
 module S = Spec.K256
-
-open Hacl.K256.Field
-open Hacl.K256.Scalar
-open Hacl.Impl.K256.Point
-open Hacl.Impl.K256.PointMul
-
+module SK = Hacl.Impl.K256.Sign
+module VK = Hacl.Impl.K256.Verify
 
 #set-options "--z3rlimit 50 --fuel 0 --ifuel 0"
 
-inline_for_extraction noextract
-val ecdsa_sign_r (r k:qelem) : Stack unit
-  (requires fun h ->
-    live h r /\ live h k /\ disjoint r k /\
-    qas_nat h k < S.q)
-  (ensures fun h0 _ h1 -> modifies (loc r) h0 h1 /\
-   (let _X, _Y, _Z = S.point_mul_g (qas_nat h0 k) in
-    let x = S.fmul _X (S.finv _Z) in
-    let r_s = x % S.q in
-    qas_nat h1 r == r_s))
-
-let ecdsa_sign_r r k =
-  push_frame ();
-  let tmp = create_felem () in
-  let p = create_point () in
-  point_mul_g p k; // p = [k]G
-  let x, y, z = getx p, gety p, getz p in
-
-  finv tmp z; // tmp = zinv
-  fmul tmp x tmp; // tmp = aff_x = x *% zinv
-  qelem_from_felem r tmp; // r = aff_x % S.q
-  pop_frame ()
-
-
-inline_for_extraction noextract
-val ecdsa_sign_s (s k r:qelem) (m private_key:lbytes32) : Stack unit
-  (requires fun h ->
-    live h s /\ live h m /\ live h private_key /\
-    live h k /\ live h r /\
-    disjoint s r /\ disjoint s k /\ disjoint r k /\
-
-    0 < qas_nat h k /\ qas_nat h k < S.q /\
-    qas_nat h r < S.q /\
-   (let d_a = BSeq.nat_from_bytes_be (as_seq h private_key) in
-    0 < d_a /\ d_a < S.q))
-  (ensures fun h0 _ h1 -> modifies (loc s) h0 h1 /\
-   (let z = BSeq.nat_from_bytes_be (as_seq h0 m) % S.q in
-    let d_a = BSeq.nat_from_bytes_be (as_seq h0 private_key) in
-    let kinv = S.qinv (qas_nat h0 k) in
-    let s_s = S.qmul kinv (S.qadd z (S.qmul (qas_nat h0 r) d_a)) in
-    qas_nat h1 s == s_s))
-
-let ecdsa_sign_s s k r m private_key =
-  push_frame ();
-  let z = create_qelem () in
-  let d_a = create_qelem () in
-  let kinv = create_qelem () in
-
-  load_qelem_modq z m; // z = m % S.q
-  load_qelem d_a private_key; // d_a = private_key
-  qinv kinv k;
-
-  qmul s r d_a; // s = r * d_a
-  qadd s z s; // s = z + s
-  qmul s kinv s; // s = kinv * s
-  pop_frame ()
-
-
 [@CInline]
 let ecdsa_sign_hashed_msg r s m private_key k =
-  push_frame ();
-  let r_q = create_qelem () in
-  let s_q = create_qelem () in
-  let k_q = create_qelem () in
-
-  load_qelem k_q k;
-  ecdsa_sign_r r_q k_q;
-  ecdsa_sign_s s_q k_q r_q m private_key;
-
-  store_qelem r r_q;
-  store_qelem s s_q;
-
-  let is_r_zero = is_qelem_zero_vartime r_q in
-  let is_s_zero = is_qelem_zero_vartime s_q in
-  let b =  if is_r_zero || is_s_zero then false else true in
-  pop_frame ();
-  b
+  SK.ecdsa_sign_hashed_msg r s m private_key k
 
 
-inline_for_extraction noextract
-val is_public_key_valid (pk_x pk_y:lbytes32) (fpk_x fpk_y:felem) : Stack bool
-  (requires fun h ->
-    live h pk_x /\ live h pk_y /\ live h fpk_x /\ live h fpk_y /\
-    disjoint fpk_x fpk_y /\ disjoint fpk_x pk_x /\ disjoint fpk_x pk_y /\
-    disjoint fpk_y pk_y /\ disjoint fpk_y pk_x)
-  (ensures  fun h0 b h1 -> modifies (loc fpk_x |+| loc fpk_y) h0 h1 /\
-    (as_nat h1 fpk_x, as_nat h1 fpk_y, b) ==
-      S.is_public_key_valid (as_seq h0 pk_x) (as_seq h0 pk_y))
-
-let is_public_key_valid pk_x pk_y fpk_x fpk_y =
-  let is_x_valid = load_felem_vartime fpk_x pk_x in
-  let is_y_valid = load_felem_vartime fpk_y pk_y in
-
-  let is_xy_on_curve =
-    if is_x_valid && is_y_valid then
-      is_on_curve_vartime fpk_x fpk_y
-    else false in
-  is_xy_on_curve
-
-
-inline_for_extraction noextract
-val ecdsa_verify_qelem (res p:point) (z r s:qelem) : Stack unit
-  (requires fun h ->
-    live h res /\ live h p /\ live h z /\ live h r /\ live h s /\
-    disjoint res p /\ point_inv h p /\
-    qas_nat h z < S.q /\ qas_nat h r < S.q /\ qas_nat h s < S.q)
-  (ensures  fun h0 _ h1 -> modifies (loc res) h0 h1 /\ point_inv h1 res /\
-    (let sinv = S.qinv (qas_nat h0 s) in
-     let u1 = S.qmul (qas_nat h0 z) sinv in
-     let u2 = S.qmul (qas_nat h0 r) sinv in
-     S.to_aff_point (point_as_nat3_proj h1 res) ==
-     S.to_aff_point (S.point_mul_double_g u1 u2 (point_as_nat3_proj h0 p))))
-
-let ecdsa_verify_qelem res p z r s =
-  push_frame ();
-  let sinv = create_qelem () in
-  let u1 = create_qelem () in
-  let u2 = create_qelem () in
-
-  qinv sinv s;
-  qmul u1 z sinv;
-  qmul u2 r sinv;
-  point_mul_g_double_vartime res u1 u2 p;
-  pop_frame ()
-
-
-inline_for_extraction noextract
-val ecdsa_verify_qelem_aff (pk_x pk_y:felem) (z r s:qelem) : Stack bool
-  (requires fun h ->
-    live h pk_x /\ live h pk_y /\ live h z /\ live h r /\ live h s /\
-    qas_nat h z < S.q /\ qas_nat h r < S.q /\ qas_nat h s < S.q /\
-    fe_lt_prime h pk_x /\ fe_lt_prime h pk_y)
-  (ensures  fun h0 b h1 -> modifies0 h0 h1 /\
-    (let sinv = S.qinv (qas_nat h0 s) in
-     let u1 = S.qmul (qas_nat h0 z) sinv in
-     let u2 = S.qmul (qas_nat h0 r) sinv in
-     let p = (as_nat h0 pk_x, as_nat h0 pk_y, S.one) in
-     let _X, _Y, _Z = S.point_mul_double_g u1 u2 p in
-     b = (S.fmul _X (S.finv _Z) % S.q = (qas_nat h0 r))))
-
-let ecdsa_verify_qelem_aff pk_x pk_y z r s =
-  push_frame ();
-  let p = create_point () in
-  let res = create_point () in
-  let zinv = create_felem () in
-  let xq = create_qelem () in
-
-  to_proj_point p pk_x pk_y;
-  ecdsa_verify_qelem res p z r s;
-  let _X, _Y, _Z = getx res, gety res, getz res in
-
-  finv zinv _Z;
-  fmul zinv _X zinv;
-  qelem_from_felem xq zinv;
-  let b = is_qelem_eq_vartime xq r in
-  pop_frame ();
-  b
-
-#push-options "--z3rlimit 150"
 [@CInline]
 let ecdsa_verify_hashed_msg m public_key_x public_key_y r s =
-  push_frame ();
-  let pk_x = create_felem () in
-  let pk_y = create_felem () in
-
-  let r_q = create_qelem () in
-  let s_q = create_qelem () in
-  let z = create_qelem () in
-
-  let is_xy_on_curve = is_public_key_valid public_key_x public_key_y pk_x pk_y in
-  let is_r_valid = load_qelem_vartime r_q r in
-  let is_s_valid = load_qelem_vartime s_q s in
-  load_qelem_modq z m;
-
-  let res =
-    if not (is_xy_on_curve && is_r_valid && is_s_valid) then false
-    else ecdsa_verify_qelem_aff pk_x pk_y z r_q s_q in
-  pop_frame ();
-  res
-#pop-options
+  VK.ecdsa_verify_hashed_msg m public_key_x public_key_y r s
 
 
 [@CInline]
