code/k256/Hacl.Impl.K256.Sign.fst
@@ -1,0 +1,117 @@
+module Hacl.Impl.K256.Sign
+
+open FStar.HyperStack
+open FStar.HyperStack.ST
+open FStar.Mul
+
+open Lib.IntTypes
+open Lib.Buffer
+
+module ST = FStar.HyperStack.ST
+module LSeq = Lib.Sequence
+module BSeq = Lib.ByteSequence
+
+module BD = Hacl.Bignum.Definitions
+
+module S = Spec.K256
+
+open Hacl.K256.Field
+open Hacl.K256.Scalar
+open Hacl.Impl.K256.Point
+open Hacl.Impl.K256.PointMul
+
+#set-options "--z3rlimit 50 --fuel 0 --ifuel 0"
+
+inline_for_extraction noextract
+let lbytes32 = lbuffer uint8 32ul
+
+inline_for_extraction noextract
+val ecdsa_sign_r (r k:qelem) : Stack unit
+  (requires fun h ->
+    live h r /\ live h k /\ disjoint r k /\
+    qas_nat h k < S.q)
+  (ensures fun h0 _ h1 -> modifies (loc r) h0 h1 /\
+   (let _X, _Y, _Z = S.point_mul_g (qas_nat h0 k) in
+    let x = S.fmul _X (S.finv _Z) in
+    let r_s = x % S.q in
+    qas_nat h1 r == r_s))
+
+let ecdsa_sign_r r k =
+  push_frame ();
+  let tmp = create_felem () in
+  let p = create_point () in
+  point_mul_g p k; // p = [k]G
+  let x, y, z = getx p, gety p, getz p in
+
+  finv tmp z; // tmp = zinv
+  fmul tmp x tmp; // tmp = aff_x = x *% zinv
+  qelem_from_felem r tmp; // r = aff_x % S.q
+  pop_frame ()
+
+
+inline_for_extraction noextract
+val ecdsa_sign_s (s k r:qelem) (m private_key:lbytes32) : Stack unit
+  (requires fun h ->
+    live h s /\ live h m /\ live h private_key /\
+    live h k /\ live h r /\
+    disjoint s r /\ disjoint s k /\ disjoint r k /\
+
+    0 < qas_nat h k /\ qas_nat h k < S.q /\
+    qas_nat h r < S.q /\
+   (let d_a = BSeq.nat_from_bytes_be (as_seq h private_key) in
+    0 < d_a /\ d_a < S.q))
+  (ensures fun h0 _ h1 -> modifies (loc s) h0 h1 /\
+   (let z = BSeq.nat_from_bytes_be (as_seq h0 m) % S.q in
+    let d_a = BSeq.nat_from_bytes_be (as_seq h0 private_key) in
+    let kinv = S.qinv (qas_nat h0 k) in
+    let s_s = S.qmul kinv (S.qadd z (S.qmul (qas_nat h0 r) d_a)) in
+    qas_nat h1 s == s_s))
+
+let ecdsa_sign_s s k r m private_key =
+  push_frame ();
+  let z = create_qelem () in
+  let d_a = create_qelem () in
+  let kinv = create_qelem () in
+
+  load_qelem_modq z m; // z = m % S.q
+  load_qelem d_a private_key; // d_a = private_key
+  qinv kinv k;
+
+  qmul s r d_a; // s = r * d_a
+  qadd s z s; // s = z + s
+  qmul s kinv s; // s = kinv * s
+  pop_frame ()
+
+
+inline_for_extraction noextract
+val ecdsa_sign_hashed_msg (r s m private_key k:lbytes32) : Stack bool
+  (requires fun h ->
+    live h m /\ live h private_key /\ live h k /\
+    live h r /\ live h s /\ disjoint r s /\
+
+   (let sk_nat = BSeq.nat_from_bytes_be (as_seq h private_key) in
+    let k_nat = BSeq.nat_from_bytes_be (as_seq h k) in
+    0 < sk_nat /\ sk_nat < S.q /\ 0 < k_nat /\ k_nat < S.q))
+  (ensures fun h0 b h1 -> modifies (loc r |+| loc s) h0 h1 /\
+    (let (r_s, s_s, b_s) =
+      S.ecdsa_sign_hashed_msg (as_seq h0 m) (as_seq h0 private_key) (as_seq h0 k) in
+     as_seq h1 r == r_s /\ as_seq h1 s == s_s /\ b == b_s))
+
+let ecdsa_sign_hashed_msg r s m private_key k =
+  push_frame ();
+  let r_q = create_qelem () in
+  let s_q = create_qelem () in
+  let k_q = create_qelem () in
+
+  load_qelem k_q k;
+  ecdsa_sign_r r_q k_q;
+  ecdsa_sign_s s_q k_q r_q m private_key;
+
+  store_qelem r r_q;
+  store_qelem s s_q;
+
+  let is_r_zero = is_qelem_zero_vartime r_q in
+  let is_s_zero = is_qelem_zero_vartime s_q in
+  let b =  if is_r_zero || is_s_zero then false else true in
+  pop_frame ();
+  b
