code/k256/Hacl.Impl.K256.Verify.fst
@@ -1,0 +1,138 @@
+module Hacl.Impl.K256.Verify
+
+open FStar.HyperStack
+open FStar.HyperStack.ST
+open FStar.Mul
+
+open Lib.IntTypes
+open Lib.Buffer
+
+module ST = FStar.HyperStack.ST
+module LSeq = Lib.Sequence
+module BSeq = Lib.ByteSequence
+
+module BD = Hacl.Bignum.Definitions
+
+module S = Spec.K256
+
+open Hacl.K256.Field
+open Hacl.K256.Scalar
+open Hacl.Impl.K256.Point
+open Hacl.Impl.K256.PointMul
+
+
+#set-options "--z3rlimit 50 --fuel 0 --ifuel 0"
+
+inline_for_extraction noextract
+let lbytes32 = lbuffer uint8 32ul
+
+inline_for_extraction noextract
+val is_public_key_valid (pk_x pk_y:lbytes32) (fpk_x fpk_y:felem) : Stack bool
+  (requires fun h ->
+    live h pk_x /\ live h pk_y /\ live h fpk_x /\ live h fpk_y /\
+    disjoint fpk_x fpk_y /\ disjoint fpk_x pk_x /\ disjoint fpk_x pk_y /\
+    disjoint fpk_y pk_y /\ disjoint fpk_y pk_x)
+  (ensures  fun h0 b h1 -> modifies (loc fpk_x |+| loc fpk_y) h0 h1 /\
+    (as_nat h1 fpk_x, as_nat h1 fpk_y, b) ==
+      S.is_public_key_valid (as_seq h0 pk_x) (as_seq h0 pk_y))
+
+let is_public_key_valid pk_x pk_y fpk_x fpk_y =
+  let is_x_valid = load_felem_vartime fpk_x pk_x in
+  let is_y_valid = load_felem_vartime fpk_y pk_y in
+
+  let is_xy_on_curve =
+    if is_x_valid && is_y_valid then
+      is_on_curve_vartime fpk_x fpk_y
+    else false in
+  is_xy_on_curve
+
+
+inline_for_extraction noextract
+val ecdsa_verify_qelem (res p:point) (z r s:qelem) : Stack unit
+  (requires fun h ->
+    live h res /\ live h p /\ live h z /\ live h r /\ live h s /\
+    disjoint res p /\ point_inv h p /\
+    qas_nat h z < S.q /\ qas_nat h r < S.q /\ qas_nat h s < S.q)
+  (ensures  fun h0 _ h1 -> modifies (loc res) h0 h1 /\ point_inv h1 res /\
+   (let sinv = S.qinv (qas_nat h0 s) in
+    let u1 = S.qmul (qas_nat h0 z) sinv in
+    let u2 = S.qmul (qas_nat h0 r) sinv in
+    S.to_aff_point (point_as_nat3_proj h1 res) ==
+    S.to_aff_point (S.point_mul_double_g u1 u2 (point_as_nat3_proj h0 p))))
+
+let ecdsa_verify_qelem res p z r s =
+  push_frame ();
+  let sinv = create_qelem () in
+  let u1 = create_qelem () in
+  let u2 = create_qelem () in
+
+  qinv sinv s;
+  qmul u1 z sinv;
+  qmul u2 r sinv;
+  point_mul_g_double_vartime res u1 u2 p;
+  pop_frame ()
+
+
+inline_for_extraction noextract
+val ecdsa_verify_qelem_aff (pk_x pk_y:felem) (z r s:qelem) : Stack bool
+  (requires fun h ->
+    live h pk_x /\ live h pk_y /\ live h z /\ live h r /\ live h s /\
+    qas_nat h z < S.q /\ qas_nat h r < S.q /\ qas_nat h s < S.q /\
+    fe_lt_prime h pk_x /\ fe_lt_prime h pk_y)
+  (ensures  fun h0 b h1 -> modifies0 h0 h1 /\
+   (let sinv = S.qinv (qas_nat h0 s) in
+    let u1 = S.qmul (qas_nat h0 z) sinv in
+    let u2 = S.qmul (qas_nat h0 r) sinv in
+    let p = (as_nat h0 pk_x, as_nat h0 pk_y, S.one) in
+    let _X, _Y, _Z = S.point_mul_double_g u1 u2 p in
+    b = (S.fmul _X (S.finv _Z) % S.q = (qas_nat h0 r))))
+
+let ecdsa_verify_qelem_aff pk_x pk_y z r s =
+  push_frame ();
+  let p = create_point () in
+  let res = create_point () in
+  let zinv = create_felem () in
+  let xq = create_qelem () in
+
+  to_proj_point p pk_x pk_y;
+  ecdsa_verify_qelem res p z r s;
+  let _X, _Y, _Z = getx res, gety res, getz res in
+
+  finv zinv _Z;
+  fmul zinv _X zinv;
+  qelem_from_felem xq zinv;
+  let b = is_qelem_eq_vartime xq r in
+  pop_frame ();
+  b
+
+
+inline_for_extraction noextract
+val ecdsa_verify_hashed_msg (m public_key_x public_key_y r s:lbytes32) : Stack bool
+  (requires fun h ->
+    live h m /\ live h public_key_x /\ live h public_key_y /\
+    live h r /\ live h s /\ disjoint r s)
+  (ensures fun h0 b h1 -> modifies0 h0 h1 /\
+    b == S.ecdsa_verify_hashed_msg (as_seq h0 m)
+      (as_seq h0 public_key_x) (as_seq h0 public_key_y) (as_seq h0 r) (as_seq h0 s))
+
+#push-options "--z3rlimit 150"
+let ecdsa_verify_hashed_msg m public_key_x public_key_y r s =
+  push_frame ();
+  let pk_x = create_felem () in
+  let pk_y = create_felem () in
+
+  let r_q = create_qelem () in
+  let s_q = create_qelem () in
+  let z = create_qelem () in
+
+  let is_xy_on_curve = is_public_key_valid public_key_x public_key_y pk_x pk_y in
+  let is_r_valid = load_qelem_vartime r_q r in
+  let is_s_valid = load_qelem_vartime s_q s in
+  load_qelem_modq z m;
+
+  let res =
+    if not (is_xy_on_curve && is_r_valid && is_s_valid) then false
+    else ecdsa_verify_qelem_aff pk_x pk_y z r_q s_q in
+  pop_frame ();
+  res
+#pop-options
